powerpc/ValueAOp.v
@@ -11,6 +11,7 @@
 (* *********************************************************************)
 
 Require Import Coqlib.
+Require Import Compopts.
 Require Import AST.
 Require Import Integers.
 Require Import Floats.
